[data] Update jenkins function
Now uses data/utilties. Also offers variants of the hash function
specialized to certain types.

books/kestrel/data/hash/jenkins.lisp
@@ -1,4 +1,4 @@
-; Copyright (C) 2025-2026 by Kestrel Institute
+; Copyright (C) 2025 by Kestrel Institute
 ;
 ; License: A 3-clause BSD license. See the LICENSE file distributed with ACL2.
 ;
@@ -13,44 +13,33 @@
 (include-book "xdoc/constructors" :dir :system)
 (include-book "xdoc/defxdoc-plus" :dir :system)
 
-(include-book "std/basic/two-nats-measure" :dir :system)
+(include-book "kestrel/data/utilities/fixed-size-words/fixnum" :dir :system)
+(include-book "kestrel/data/utilities/fixed-size-words/u32-defs" :dir :system)
 
-(include-book "sum-acl2-count-defs")
+(local (include-book "std/basic/controlled-configuration" :dir :system))
+(local (acl2::controlled-configuration :hooks nil))
 
-(local (include-book "kestrel/built-ins/disable" :dir :system))
-(local (acl2::disable-most-builtin-logic-defuns))
-(local (acl2::disable-builtin-rewrite-rules-for-defaults))
-(set-induction-depth-limit 0)
+(local (include-book "kestrel/data/utilities/fixed-size-words/u32" :dir :system))
+(local (include-book "kestrel/data/utilities/bit-vectors/bitops" :dir :system))
 
 (local (include-book "kestrel/arithmetic-light/ash" :dir :system))
-(local (include-book "kestrel/arithmetic-light/fix" :dir :system))
-(local (include-book "kestrel/arithmetic-light/minus" :dir :system))
-(local (include-book "kestrel/arithmetic-light/mod" :dir :system))
-(local (include-book "kestrel/arithmetic-light/natp" :dir :system))
-(local (include-book "kestrel/arithmetic-light/plus" :dir :system))
-(local (include-book "kestrel/arithmetic-light/plus-and-minus" :dir :system))
 
-(local (include-book "kestrel/bv/logand" :dir :system))
-(local (include-book "kestrel/bv/logxor" :dir :system))
 (local (include-book "kestrel/bv/unsigned-byte-p" :dir :system))
-
-(local (include-book "kestrel/lists-light/len" :dir :system))
 
 (local (include-book "kestrel/strings-light/char" :dir :system))
 
 (local (include-book "kestrel/utilities/nfix" :dir :system))
-
-(local (include-book "sum-acl2-count"))
-
-;;;;;;;;;;;;;;;;;;;;;;;;;;;;;;;;;;;;;;;;;;;;;;;;;;;;;;;;;;;;;;;;;;;;;;;;;;;;;;;;
-
-(std::make-define-config
-  :no-function t)
+(local (include-book "kestrel/utilities/ordinals" :dir :system))
 
 ;;;;;;;;;;;;;;;;;;;;;;;;;;;;;;;;;;;;;;;;;;;;;;;;;;;;;;;;;;;;;;;;;;;;;;;;;;;;;;;;
 
-(defxdoc+ jenkins-hash
-  :parents (implementation)
+;; We don't seem to have good rules about logtail
+(local (in-theory (disable acl2::right-shift-to-logtail)))
+
+;;;;;;;;;;;;;;;;;;;;;;;;;;;;;;;;;;;;;;;;;;;;;;;;;;;;;;;;;;;;;;;;;;;;;;;;;;;;;;;;
+
+(defxdoc+ jenkins-one-at-a-time
+  :parents (hashes)
   :short
   (xdoc::topstring
     "An implementation of "
@@ -67,7 +56,7 @@
       "The implementation is similar to @('acl2::fchecksum-obj') (see @(see
        acl2::checksum)) in how we collect input bytes for the hash while
        walking over the ACL2 object.")
-    (xdoc::@def "jenkins-hash")
+    (xdoc::@def "jenkins")
     (xdoc::section
       "References"
       (xdoc::ul
@@ -86,52 +75,27 @@
 
 ;;;;;;;;;;;;;;;;;;;;;;;;;;;;;;;;;;;;;;;;;;;;;;;;;;;;;;;;;;;;;;;;;;;;;;;;;;;;;;;;
 
-(defconst *u8-max*
-  (- (expt 2 8) 1))
-
-(defconst *u32-max*
-  (- (expt 2 32) 1))
-
-(defconst *u-fixnum-max*
-  (- (expt 2 acl2::*fixnum-bits*) 1))
-
-;;;;;;;;;;;;;;;;;;;;;;;;;;;;;;;;;;;;;;;;;;;;;;;;;;;;;;;;;;;;;;;;;;;;;;;;;;;;;;;;
-
-(define u32-+ (x y)
-  (declare (type (unsigned-byte 32) x)
-           (type (unsigned-byte 32) y)
-           (xargs :type-prescription (natp (u32-+ x y)))
-           (optimize (speed 3) (safety 0)))
-  :returns (product (unsigned-byte-p 32 product))
-  (the (unsigned-byte 32)
-    (logand (+ x y)
-            *u32-max*))
-  :inline t)
-
-(define u32-ash (i c)
-  (declare (type (unsigned-byte 32) i)
-           (type (integer -31 31) c)
-           (xargs :type-prescription (natp (u32-ash i c)))
-           (optimize (speed 3) (safety 0)))
-  :returns (shift (unsigned-byte-p 32 shift))
-  (the (unsigned-byte 32)
-    (logand (ash i c)
-            *u32-max*))
-  :inline t)
-
-;;;;;;;;;;;;;;;;;;;;;;;;;;;;;;;;;;;;;;;;;;;;;;;;;;;;;;;;;;;;;;;;;;;;;;;;;;;;;;;;
-
-(define jenkins-acc-byte (byte acc)
-  (declare (type (unsigned-byte 8) byte)
-           (type (unsigned-byte 32) acc)
-           (xargs :type-prescription (natp (jenkins-acc-byte byte acc)))
-           (optimize (speed 3) (safety 0)))
+(define jenkins-acc-byte
+  ((byte (unsigned-byte-p 8 byte))
+   (acc (unsigned-byte-p 32 acc)))
+  (declare (xargs :split-types t)
+           (type (unsigned-byte 8) byte)
+           (type (unsigned-byte 32) acc))
   :returns (acc$ (unsigned-byte-p 32 acc$))
   (the (unsigned-byte 32)
-    (let* ((acc (u32-+ acc byte))
-           (acc (u32-+ acc (u32-ash acc 10))))
-      (logxor acc (u32-ash acc -6))))
+    (let* ((acc (data::u32-plus acc byte))
+           (acc (data::u32-plus acc (data::u32-shl acc 10))))
+      (data::u32-xor acc (data::u32-shr acc 6))))
   :inline t)
+
+;;;;;;;;;;;;;;;;;;;;;;;;;;;;;;;;;;;;;;;;
+
+(in-theory (disable (:t jenkins-acc-byte)))
+
+(defrule jenkins-acc-byte-type-prescription
+  (natp (jenkins-acc-byte byte acc))
+  :rule-classes :type-prescription
+  :enable jenkins-acc-byte)
 
 ;;;;;;;;;;;;;;;;;;;;;;;;;;;;;;;;;;;;;;;;;;;;;;;;;;;;;;;;;;;;;;;;;;;;;;;;;;;;;;;;
 
@@ -139,43 +103,59 @@
 
 ;;;;;;;;;;;;;;;;;;;;;;;;;;;;;;;;;;;;;;;;
 
-(define jenkins-acc-character (c acc)
-  (declare (type character c)
-           (type (unsigned-byte 32) acc)
-           (xargs :type-prescription (natp (jenkins-acc-character c acc)))
-           (optimize (speed 3) (safety 0)))
+(define jenkins-acc-character
+  ((c characterp)
+   (acc (unsigned-byte-p 32 acc)))
+  (declare (xargs :split-types t)
+           (type character c)
+           (type (unsigned-byte 32) acc))
   :returns (acc$ (unsigned-byte-p 32 acc$))
   (the (unsigned-byte 32)
     (jenkins-acc-byte (the (unsigned-byte 8)
                         (char-code c))
                       acc))
-  :inline t)
+  :inline t
+  :guard-hints (("Goal" :in-theory (enable unsigned-byte-p
+                                           integer-range-p))))
+
+(in-theory (disable (:t jenkins-acc-character)))
+
+(defrule jenkins-acc-character-type-prescription
+  (natp (jenkins-acc-character c acc))
+  :rule-classes :type-prescription
+  :enable jenkins-acc-character)
 
 ;;;;;;;;;;;;;;;;;;;;;;;;;;;;;;;;;;;;;;;;
 
-;; TODO: use loop$ (here and elsewhere)
-(define jenkins-acc-string-fixnum-index (str i len acc)
-  :guard (and (<= i len)
-              (equal len (length str)))
-  (declare (type string str)
-           (type #.*u-fixnum-type* i)
-           (type #.*u-fixnum-type* len)
-           (type (unsigned-byte 32) acc)
-           (optimize (speed 3) (safety 0)))
+;; TODO: use loop$
+(define jenkins-acc-string-fixnum-index
+  ((str stringp)
+   (i (unsigned-byte-p data::*fixnum-bits* i))
+   (len (unsigned-byte-p data::*fixnum-bits* len))
+   (acc (unsigned-byte-p 32 acc)))
+  :guard (mbe :logic (and (<= i len)
+                          (equal len (length str)))
+              :exec (and (<= (data::the-u-fixnum i)
+                             (data::the-u-fixnum len))
+                         (equal (data::the-u-fixnum len)
+                                (length (the string str)))))
+  (declare (xargs :split-types t)
+           (type string str)
+           (type #.data::*u-fixnum-type* i len)
+           (type (unsigned-byte 32) acc))
   :returns (acc$ (unsigned-byte-p 32 acc$))
   (let ((i (mbe :logic (nfix i)
                 :exec i))
         (len (mbe :logic (nfix len)
                   :exec len)))
     ;; TODO: redundant?
-    (declare (type #.*u-fixnum-type* i)
-             (type #.*u-fixnum-type* len))
+    (declare (type #.data::*u-fixnum-type* i len))
     (if (and (mbt (and (<= i len)
-                       (<= len *u-fixnum-max*)))
+                       (<= len #.data::*u-fixnum-max*)))
              (< i len))
         (jenkins-acc-string-fixnum-index
           str
-          (the #.*u-fixnum-type* (1+ i))
+          (the #.data::*u-fixnum-type* (1+ i))
           len
           (jenkins-acc-character (the character (char str i)) acc))
       (mbe :logic (if (unsigned-byte-p 32 acc)
@@ -183,12 +163,9 @@
                     0)
            :exec acc)))
   :measure (nfix (- len (nfix i)))
-  :hints (("Goal" :in-theory (enable o-p
-                                     o<
-                                     o-finp
-                                     nfix
-                                     natp
-                                     the-check))))
+  :hints (("Goal" :in-theory (enable the-check))))
+
+(in-theory (disable (:t jenkins-acc-string-fixnum-index)))
 
 (defrule jenkins-acc-string-fixnum-index-type-prescription
   (natp (jenkins-acc-string-fixnum-index str i len acc))
@@ -196,22 +173,27 @@
   :induct t
   :enable jenkins-acc-string-fixnum-index)
 
-(define jenkins-acc-string-nonfixnum-index (str i len acc)
-  :guard (and (<= i len)
-              (equal len (length str)))
-  (declare (type string str)
+(define jenkins-acc-string-nonfixnum-index
+  ((str stringp)
+   (i natp)
+   (len natp)
+   (acc (unsigned-byte-p 32 acc)))
+  :guard (mbe :logic (and (<= i len)
+                          (equal len (length str)))
+              :exec (and (<= (the unsigned-byte i) (the unsigned-byte len))
+                         (equal (the unsigned-byte len) (length str))))
+  (declare (xargs :split-types t)
+           (type string str)
            (type unsigned-byte i)
            (type unsigned-byte len)
-           (type (unsigned-byte 32) acc)
-           (optimize (speed 3) (safety 0)))
+           (type (unsigned-byte 32) acc))
   :returns (acc$ (unsigned-byte-p 32 acc$))
   (let ((i (mbe :logic (nfix i)
                 :exec i))
         (len (mbe :logic (nfix len)
                   :exec len)))
     ;; TODO: redundant?
-    (declare (type unsigned-byte i)
-             (type unsigned-byte len))
+    (declare (type unsigned-byte i len))
     (if (and (mbt (<= i len))
              (< i len))
         (jenkins-acc-string-nonfixnum-index
@@ -224,12 +206,7 @@
                     0)
            :exec acc)))
   :measure (nfix (- len (nfix i)))
-  :hints (("Goal" :in-theory (enable o-p
-                                     o<
-                                     o-finp
-                                     nfix
-                                     natp
-                                     the-check))))
+  :hints (("Goal" :in-theory (enable the-check))))
 
 (defrule jenkins-acc-string-nonfixnum-index-type-prescription
   (natp (jenkins-acc-string-nonfixnum-index str i len acc))
@@ -238,84 +215,118 @@
   :enable jenkins-acc-string-nonfixnum-index)
 
 (define jenkins-acc-string
-  (str acc)
-  (declare (type string str)
-           (type (unsigned-byte 32) acc)
-           (xargs :type-prescription (natp (jenkins-acc-string str acc)))
-           (optimize (speed 3) (safety 0)))
+  ((str stringp)
+   (acc (unsigned-byte-p 32 acc)))
+  (declare (xargs :split-types t)
+           (type string str)
+           (type (unsigned-byte 32) acc))
   :returns (acc$ (unsigned-byte-p 32 acc$))
   (the (unsigned-byte 32)
     (let ((len (length str)))
       (declare (type unsigned-byte len))
-      (if (<= len *u-fixnum-max*)
-          (jenkins-acc-string-fixnum-index str 0 (the #.*u-fixnum-type* len) acc)
+      (if (<= len #.data::*u-fixnum-max*)
+          (jenkins-acc-string-fixnum-index str 0 (data::the-u-fixnum len) acc)
         (jenkins-acc-string-nonfixnum-index str 0 len acc))))
   :inline t)
 
+(in-theory (disable (:t jenkins-acc-string)))
+
+(defrule jenkins-acc-string-type-prescription
+  (natp (jenkins-acc-string str acc))
+  :rule-classes :type-prescription
+  :enable jenkins-acc-string)
+
 ;;;;;;;;;;;;;;;;;;;;;;;;;;;;;;;;;;;;;;;;
 
-(define jenkins-acc-nat (n acc)
-  (declare (type unsigned-byte n)
-           (type (unsigned-byte 32) acc)
-           (xargs :type-prescription (natp (jenkins-acc-nat n acc)))
-           (optimize (speed 3) (safety 0)))
+(define jenkins-acc-nat
+  ((n natp)
+   (acc (unsigned-byte-p 32 acc)))
+  (declare (xargs :split-types t)
+           (type unsigned-byte n)
+           (type (unsigned-byte 32) acc))
   :returns (acc$ (unsigned-byte-p 32 acc$))
   (if (or (not (mbt (natp n)))
-          (< n *u8-max*))
+          (< n #.data::*u8-max*))
       (jenkins-acc-byte (the (unsigned-byte 8) n) acc)
     (jenkins-acc-nat (the unsigned-byte (ash n -8))
                      (jenkins-acc-byte (the (unsigned-byte 8)
-                                         (logand n *u8-max*))
+                                         (logand n #.data::*u8-max*))
                                        acc)))
   :measure (nfix n)
-  :hints (("Goal" :in-theory (enable o-p
-                                     o<
-                                     o-finp
-                                     nfix
-                                     the-check))))
+  :hints (("Goal" :in-theory (enable the-check))))
 
-(define jenkins-acc-integer (n acc)
-  (declare (type signed-byte n)
-           (type (unsigned-byte 32) acc)
-           (xargs :type-prescription (natp (jenkins-acc-integer n acc)))
-           (optimize (speed 3) (safety 0)))
+(defrule jenkins-acc-nat-type-prescription
+  (natp (jenkins-acc-nat n acc))
+  :rule-classes :type-prescription
+  :enable jenkins-acc-nat)
+
+(define jenkins-acc-integer
+  ((n integerp)
+   (acc (unsigned-byte-p 32 acc)))
+  (declare (xargs :split-types t)
+           (type signed-byte n)
+           (type (unsigned-byte 32) acc))
   :returns (acc$ (unsigned-byte-p 32 acc$))
   (the (unsigned-byte 32)
     (if (natp n)
         (jenkins-acc-nat n acc)
       (jenkins-acc-nat (the unsigned-byte (- n))
-                  (jenkins-acc-byte 0 acc))))
+                       (jenkins-acc-byte 0 acc))))
   :inline t)
 
-(define jenkins-acc-rational (n acc)
-  (declare (type rational n)
-           (type (unsigned-byte 32) acc)
-           (xargs :type-prescription (natp (jenkins-acc-rational n acc)))
-           (optimize (speed 3) (safety 0)))
+(in-theory (disable (:t jenkins-acc-integer)))
+
+(defrule jenkins-acc-integer-type-prescription
+  (natp (jenkins-acc-integer n acc))
+  :rule-classes :type-prescription
+  :enable jenkins-acc-integer)
+
+(define jenkins-acc-rational
+  ((n rationalp)
+   (acc (unsigned-byte-p 32 acc)))
+  (declare (xargs :split-types t)
+           (type rational n)
+           (type (unsigned-byte 32) acc))
   :returns (acc$ (unsigned-byte-p 32 acc$))
   (the (unsigned-byte 32)
     (jenkins-acc-nat (denominator n)
-                (jenkins-acc-integer (numerator n)
-                                acc)))
+                     (jenkins-acc-integer (numerator n)
+                                          acc)))
   :inline t)
 
-(define jenkins-acc-complex-rational (n acc)
-  (declare (type complex n)
-           (type (unsigned-byte 32) acc)
-           (xargs :type-prescription (natp (jenkins-acc-complex-rational n acc)))
-           (optimize (speed 3) (safety 0)))
+(in-theory (disable (:t jenkins-acc-rational)))
+
+(defrule jenkins-acc-rational-type-prescription
+  (natp (jenkins-acc-rational n acc))
+  :rule-classes :type-prescription
+  :enable jenkins-acc-rational)
+
+(define jenkins-acc-complex-rational
+  ((n complex-rationalp)
+   (acc (unsigned-byte-p 32 acc)))
+  (declare (xargs :split-types t)
+           (type complex n)
+           (type (unsigned-byte 32) acc))
   :returns (acc$ (unsigned-byte-p 32 acc$))
   (the (unsigned-byte 32)
     (jenkins-acc-rational (imagpart n)
-                     (jenkins-acc-rational (realpart n)
-                                      acc)))
+                          (jenkins-acc-rational (realpart n)
+                                                acc)))
   :inline t)
 
-(define jenkins-acc-acl2-number (n acc)
-  (declare (type number n)
-           (type (unsigned-byte 32) acc)
-           (xargs :type-prescription (natp (jenkins-acc-acl2-number n acc)))
-           (optimize (speed 3) (safety 0)))
+(in-theory (disable (:t jenkins-acc-complex-rational)))
+
+(defrule jenkins-acc-complex-rational-type-prescription
+  (natp (jenkins-acc-complex-rational n acc))
+  :rule-classes :type-prescription
+  :enable jenkins-acc-complex-rational)
+
+(define jenkins-acc-acl2-number
+  ((n acl2-numberp)
+   (acc (unsigned-byte-p 32 acc)))
+  (declare (xargs :split-types t)
+           (type number n)
+           (type (unsigned-byte 32) acc))
   :returns (acc$ (unsigned-byte-p 32 acc$))
   (the (unsigned-byte 32)
     (cond ((integerp n)
@@ -325,27 +336,45 @@
           (t (jenkins-acc-complex-rational (the complex n) acc))))
   :inline t)
 
+(in-theory (disable (:t jenkins-acc-acl2-number)))
+
+(defrule jenkins-acc-acl2-number-type-prescription
+  (natp (jenkins-acc-acl2-number n acc))
+  :rule-classes :type-prescription
+  :enable jenkins-acc-acl2-number)
+
 ;;;;;;;;;;;;;;;;;;;;;;;;;;;;;;;;;;;;;;;;
 
 (define jenkins-acc-symbol
-  (symbol acc)
-  (declare (type symbol symbol)
-           (type (unsigned-byte 32) acc)
-           (xargs :type-prescription (natp (jenkins-acc-symbol symbol acc)))
-           (optimize (speed 3) (safety 0)))
+  ((symbol symbolp)
+   (acc (unsigned-byte-p 32 acc)))
+  (declare (xargs :split-types t)
+           (type symbol symbol)
+           (type (unsigned-byte 32) acc))
   :returns (acc$ (unsigned-byte-p 32 acc$))
   (the (unsigned-byte 32)
     (jenkins-acc-string (symbol-name symbol)
-                   (jenkins-acc-string (symbol-package-name symbol)
-                                  acc)))
+                        (jenkins-acc-string (symbol-package-name symbol)
+                                            acc)))
   :inline t)
+
+(in-theory (disable (:t jenkins-acc-symbol)))
+
+(defrule jenkins-acc-symbol-type-prescription
+  (natp (jenkins-acc-symbol symbol acc))
+  :rule-classes :type-prescription
+  :enable jenkins-acc-symbol)
 
 ;;;;;;;;;;;;;;;;;;;;;;;;;;;;;;;;;;;;;;;;
 
-(define jenkins-acc-atom (x acc)
-  (declare (type atom x)
-           (type (unsigned-byte 32) acc)
-           (optimize (speed 3) (safety 0)))
+(define jenkins-acc-atom
+  (x
+   (acc (unsigned-byte-p 32 acc)))
+  :guard (mbe :logic (not (consp x))
+              :exec (atom x))
+  (declare (xargs :split-types t)
+           (type atom x)
+           (type (unsigned-byte 32) acc))
   :returns (acc$ (unsigned-byte-p 32 acc$))
   (the (unsigned-byte 32)
     (cond ((symbolp x)
@@ -361,7 +390,10 @@
                             acc
                           0)
                  :exec acc))))
-  :inline t)
+  :inline t
+  :guard-hints (("Goal" :in-theory (enable atom))))
+
+(in-theory (disable (:t jenkins-acc-atom)))
 
 (defrule jenkins-acc-atom-type-presciption
   (natp (jenkins-acc-atom list acc))
@@ -370,54 +402,99 @@
 
 ;;;;;;;;;;;;;;;;;;;;;;;;;;;;;;;;;;;;;;;;
 
-;; TODO: loop$
-;; TODO: Is this associative on cons? Hopefully not
-(define jenkins-acc-true-list
-  ((list true-listp)
-   acc)
-  (declare (type (or cons null) list)
-           (type (unsigned-byte 32) acc)
-           (optimize (speed 3) (safety 0)))
+(define jenkins-acc
+  (x
+   (acc (unsigned-byte-p 32 acc)))
+  (declare (xargs :split-types t)
+           (type (unsigned-byte 32) acc))
   :returns (acc$ (unsigned-byte-p 32 acc$))
   (let ((acc (mbe :logic (if (unsigned-byte-p 32 acc)
                              acc
                            0)
                   :exec acc)))
-    (if (endp list)
-        acc
-      (let ((first (first list)))
-        (if (consp first)
-            (jenkins-acc-true-list (list* (car first) (cdr first) (rest list))
-                                   (jenkins-acc-byte
-                                     ;; We chose an arbitrary byte to represent
-                                     ;; cons
-                                     #x70
-                                     acc))
-          (jenkins-acc-true-list (rest list)
-                                 (jenkins-acc-atom first acc))))))
-  :measure (acl2::nat-list-measure
-            (list (sum-acl2-count list)
-                  (len list)))
-  :hints (("Goal" :in-theory (enable sum-acl2-count))))
+    (if (consp x)
+        (jenkins-acc (cdr x)
+                     (jenkins-acc (car x)
+                                  (jenkins-acc-byte
+                                    ;; We chose an arbitrary byte to represent
+                                    ;; cons
+                                    #x70
+                                    acc)))
+      (jenkins-acc-atom x acc)))
+  :verify-guards :after-returns)
 
-(defrule jenkins-acc-true-list-type-presciption
-  (natp (jenkins-acc-true-list list acc))
+(in-theory (disable (:t jenkins-acc)))
+
+(defrule jenkins-acc-type-presciption
+  (natp (jenkins-acc x acc))
   :rule-classes :type-prescription
   :induct t
-  :enable jenkins-acc-true-list)
+  :enable jenkins-acc)
 
 ;;;;;;;;;;;;;;;;;;;;;;;;;;;;;;;;;;;;;;;;
 
 (define jenkins (x)
-  (declare (xargs :type-prescription (natp (jenkins x)))
-           (optimize (speed 3) (safety 0)))
+  :parents (jenkins-one-at-a-time)
   :returns (hash (unsigned-byte-p 32 hash))
-  ;; Avoid clash with XDOC topic
-  :parents nil
   (the (unsigned-byte 32)
     (let* ((acc (the (unsigned-byte 32)
-                  (jenkins-acc-true-list (list x) 0)))
-           (acc (u32-+ acc (u32-ash acc 3)))
-           (acc (the (unsigned-byte 32)
-                  (logxor acc (u32-ash acc -11)))))
-      (u32-+ acc (u32-ash acc 15)))))
+                  (jenkins-acc x 0)))
+           (acc (data::u32-plus acc (data::u32-shl acc 3)))
+           (acc (data::u32-xor acc (data::u32-shr acc 11))))
+      (data::u32-plus acc (data::u32-shl acc 15)))))
+
+(in-theory (disable (:t jenkins-acc)))
+
+(defrule jenkins-type-presciption
+  (natp (jenkins x))
+  :rule-classes :type-prescription
+  :enable jenkins)
+
+;;;;;;;;;;;;;;;;;;;;;;;;;;;;;;;;;;;;;;;;
+
+(define acl2-number-jenkins
+  ((x acl2-numberp))
+  (mbe :logic (jenkins x)
+       :exec (the (unsigned-byte 32)
+               (let* ((acc (the (unsigned-byte 32)
+                             (jenkins-acc-acl2-number x 0)))
+                      (acc (data::u32-plus acc (data::u32-shl acc 3)))
+                      (acc (data::u32-xor acc (data::u32-shr acc 11))))
+                 (data::u32-plus acc (data::u32-shl acc 15)))))
+  :enabled t
+  :guard-hints (("Goal" :in-theory (enable jenkins
+                                           jenkins-acc
+                                           jenkins-acc-atom))))
+
+(define symbol-jenkins
+  ((x symbolp))
+  (mbe :logic (jenkins x)
+       :exec (the (unsigned-byte 32)
+               (let* ((acc (the (unsigned-byte 32)
+                             (jenkins-acc-symbol x 0)))
+                      (acc (data::u32-plus acc (data::u32-shl acc 3)))
+                      (acc (data::u32-xor acc (data::u32-shr acc 11))))
+                 (data::u32-plus acc (data::u32-shl acc 15)))))
+  :enabled t
+  :guard-hints (("Goal" :in-theory (enable jenkins
+                                           jenkins-acc
+                                           jenkins-acc-atom))))
+
+(define eqlable-jenkins
+  ((x eqlablep))
+  (mbe :logic (jenkins x)
+       :exec (the (unsigned-byte 32)
+               (let* ((acc (the (unsigned-byte 32)
+                             (cond ((symbolp x)
+                                    (jenkins-acc-symbol x 0))
+                                   ((acl2-numberp x)
+                                    (jenkins-acc-acl2-number x 0))
+                                   (t
+                                    (jenkins-acc-character x 0)))))
+                      (acc (data::u32-plus acc (data::u32-shl acc 3)))
+                      (acc (data::u32-xor acc (data::u32-shr acc 11))))
+                 (data::u32-plus acc (data::u32-shl acc 15)))))
+  :enabled t
+  :guard-hints (("Goal" :in-theory (enable jenkins
+                                           jenkins-acc
+                                           jenkins-acc-atom))))
